Finishing the conversion to the one-component parity example (without composition)

theories/VLSM/Core/Examples/NewParity.v
@@ -83,8 +83,8 @@ Ltac app_valid_tran :=
 
 Section sec_parity_vlsm.
 
-Context (multiplier : nat)
-        (multiplier_geq_2 : Z.of_nat multiplier >= 2).
+Context (multiplier : Z)
+        (multiplier_geq_2 : multiplier >= 2).
 
 (** ** Definition of Parity VLSM
 
@@ -121,7 +121,7 @@ Definition ParityComponent_transition
   (l : ParityLabel) (st : ParityState) (om : option ParityMessage)
   : ParityState * option ParityMessage :=
   match om with
-  | Some j  => ((st - j), Some (Z.of_nat multiplier * j))
+  | Some j  => ((st - j), Some (multiplier * j))
   | None    => (st, None)
   end.
 
@@ -157,7 +157,7 @@ Proof. done. Defined.
 Definition ParityMachine : VLSMMachine ParityType :=
 {|
   initial_state_prop := ParityComponent_initial_state_prop;
-  initial_message_prop := fun (ms : ParityMessage) => ms = Z.of_nat multiplier;
+  initial_message_prop := fun (ms : ParityMessage) => ms = multiplier;
   s0 := ParityComponent_Inhabited_initial_state_type;
   transition := fun l '(st, om) => ParityComponent_transition l st om;
   valid := fun l '(st, om) => ParityComponentValid l st om;
@@ -178,7 +178,7 @@ Definition parity_label : label ParityVLSM := ().
 (** *** Example of an arbitrary transition *)
 
 Lemma parity_example_transition_1 `(X : VLSM message) :
-  transition ParityVLSM parity_label (4, Some 10) = (-6, Some (Z.of_nat multiplier * 10)).
+  transition ParityVLSM parity_label (4, Some 10) = (-6, Some (multiplier * 10)).
 Proof. done. Qed.
 
 (** *** Example of a valid trace *)
@@ -192,84 +192,86 @@ Proof. done. Qed.
 *)
 
 Definition parity_trace1_init : list (transition_item ParityVLSM) :=
-  [ Build_transition_item parity_label (Some (Z.of_nat multiplier ^ 2))
-                                       (Z.of_nat multiplier ^ 3 - Z.of_nat multiplier ^ 2)
-                                       (Some (Z.of_nat multiplier ^ 3))
-  ; Build_transition_item parity_label (Some (Z.of_nat multiplier))
-                                       (Z.of_nat multiplier ^ 3 - Z.of_nat multiplier ^ 2 - Z.of_nat multiplier)
-                                       (Some (Z.of_nat multiplier ^ 2)) ].
+  [ Build_transition_item parity_label (Some (multiplier ^ 2))
+                                       (multiplier ^ 3 - multiplier ^ 2)
+                                       (Some (multiplier ^ 3))
+  ; Build_transition_item parity_label (Some multiplier)
+                                       (multiplier ^ 3 - multiplier ^ 2 - multiplier)
+                                       (Some (multiplier ^ 2)) ].
 
 Definition parity_trace1_last_item : transition_item ParityVLSM :=
-  Build_transition_item parity_label (Some (Z.of_nat multiplier))
-  (Z.of_nat multiplier ^ 3 - Z.of_nat multiplier ^ 2 - Z.of_nat multiplier - Z.of_nat multiplier)
-  (Some (Z.of_nat multiplier ^ 2)).
+  Build_transition_item parity_label (Some multiplier)
+  (multiplier ^ 3 - multiplier ^ 2 - multiplier - multiplier)
+  (Some (multiplier ^ 2)).
 
 Definition parity_trace1 : list (transition_item ParityVLSM) :=
   parity_trace1_init ++ [parity_trace1_last_item].
 
-Definition parity_trace1_first_state : ParityState := Z.of_nat multiplier ^ 3.
+Definition parity_trace1_first_state : ParityState := multiplier ^ 3.
 
 Definition parity_trace1_last_state : ParityState := destination parity_trace1_last_item.
 
 (** Defined trace is valid: *)
 
-Example parity_valid_message_prop_mult : valid_message_prop ParityVLSM (Z.of_nat multiplier).
+Example parity_valid_message_prop_mult : valid_message_prop ParityVLSM (multiplier).
 Proof. by apply initial_message_is_valid. Qed.
 
-Example parity_can_emit_square_mult : can_emit ParityVLSM (Z.of_nat multiplier ^ 2).
+Example parity_can_emit_square_mult : can_emit ParityVLSM (multiplier ^ 2).
 Proof.
-  exists (Z.of_nat multiplier, Some (Z.of_nat multiplier)), parity_label, 0.
-  by repeat split; [assert (Z.of_nat multiplier >= 1) by lia; app_valid_tran.. | | lia | cbn; repeat f_equal; lia].
+  exists (multiplier, Some multiplier), parity_label, 0.
+  repeat split; [| | lia.. | cbn; do 2 f_equal; lia].
+  - by apply initial_state_is_valid; cbn; unfold ParityComponent_initial_state_prop; lia.
+  - by app_valid_tran.
 Qed.
 
-Example parity_valid_message_prop_square_mult : valid_message_prop ParityVLSM (Z.of_nat multiplier ^ 2).
+Example parity_valid_message_prop_square_mult : valid_message_prop ParityVLSM ( multiplier ^ 2).
 Proof.
-  by apply (emitted_messages_are_valid ParityVLSM (Z.of_nat multiplier ^ 2) parity_can_emit_square_mult).
+  by apply (emitted_messages_are_valid ParityVLSM (multiplier ^ 2) parity_can_emit_square_mult).
 Qed.
 
 Proposition parity_valid_transition_1 :
   input_valid_transition ParityVLSM parity_label
-   (parity_trace1_first_state, Some (Z.of_nat multiplier ^ 2))
-   (Z.of_nat multiplier ^ 3 - Z.of_nat multiplier ^ 2, Some (Z.of_nat multiplier ^ 3)).
+   (parity_trace1_first_state, Some (multiplier ^ 2))
+   (multiplier ^ 3 - multiplier ^ 2, Some (multiplier ^ 3)).
 Proof.
   repeat split; [| | | lia].
-  - apply initial_state_is_valid.
-    by assert (Z.of_nat multiplier ^ 3 >= 1) by lia.
+  - apply initial_state_is_valid; cbn;
+      unfold ParityComponent_initial_state_prop, parity_trace1_first_state; lia.
   - by app_valid_tran; apply parity_can_emit_square_mult.
-  - unfold parity_trace1_first_state. 
-    assert (Z.of_nat multiplier ^ 3 = Z.of_nat multiplier ^ 2 * Z.of_nat multiplier) by lia.
-    by rewrite H; nia.
+  - by unfold parity_trace1_first_state; nia.
 Qed.
 
 Proposition parity_valid_transition_2 :
   input_valid_transition ParityVLSM parity_label
-   (Z.of_nat multiplier ^ 3 - Z.of_nat multiplier ^ 2, Some (Z.of_nat multiplier))
-   (Z.of_nat multiplier ^ 3 - Z.of_nat multiplier ^ 2 - Z.of_nat multiplier, Some (Z.of_nat multiplier ^ 2)).
+   (multiplier ^ 3 - multiplier ^ 2, Some multiplier)
+   (multiplier ^ 3 - multiplier ^ 2 - multiplier, Some (multiplier ^ 2)).
 Proof.
   repeat split; [| | | lia |].
   - by app_valid_tran; apply parity_valid_transition_1.
   - by app_valid_tran; apply parity_can_emit_square_mult.
   - by nia.
-  - by cbn; repeat f_equal; lia.
+  - by cbn; do 2 f_equal; lia.
 Qed.
 
 Proposition parity_valid_transition_3 : 
   input_valid_transition ParityVLSM parity_label
-  (Z.of_nat multiplier ^ 3 - Z.of_nat multiplier ^ 2 - Z.of_nat multiplier, Some (Z.of_nat multiplier))
-  (Z.of_nat multiplier ^ 3 - Z.of_nat multiplier ^ 2 - Z.of_nat multiplier - Z.of_nat multiplier, Some (Z.of_nat multiplier ^ 2)).
+  (multiplier ^ 3 - multiplier ^ 2 - multiplier, Some multiplier)
+  (multiplier ^ 3 - multiplier ^ 2 - multiplier - multiplier, Some (multiplier ^ 2)).
 Proof.
   repeat split; [| | | lia |].
   - by app_valid_tran; apply parity_valid_transition_2.
   - by app_valid_tran; apply parity_can_emit_square_mult.
   - by nia.
-  - by cbn; repeat f_equal; lia.
+  - by cbn; do 2 f_equal; lia.
 Qed.
 
 Example parity_valid_trace1 :
   finite_valid_trace_init_to ParityVLSM
    parity_trace1_first_state parity_trace1_last_state parity_trace1.
 Proof.
-  constructor; [| by assert (Z.of_nat multiplier ^ 3 >= 1) by lia].
+  constructor; [| unfold parity_trace1_first_state; cbn;
+                  unfold ParityComponent_initial_state_prop; lia].
+  unfold parity_trace1_first_state.
   repeat apply finite_valid_trace_from_to_extend.
   - by eapply finite_valid_trace_from_to_empty, input_valid_transition_destination, parity_valid_transition_3.
   - by apply parity_valid_transition_3.
@@ -281,7 +283,8 @@ Example parity_valid_trace1_alt :
   finite_valid_trace_init_to_alt ParityVLSM
    parity_trace1_first_state parity_trace1_last_state parity_trace1.
 Proof.
-  constructor; [| by assert (Z.of_nat multiplier ^ 3 >= 1) by lia].
+  constructor; [| unfold parity_trace1_first_state; cbn;
+                  unfold ParityComponent_initial_state_prop; lia].
   repeat apply mvt_extend; [.. | apply mvt_empty].
   - by apply parity_valid_message_prop_square_mult.
   - by apply parity_valid_transition_1.
@@ -302,7 +305,8 @@ Lemma parity_constrained_trace1 :
   finite_constrained_trace_init_to ParityVLSM
    parity_trace1_first_state parity_trace1_last_state parity_trace1.
 Proof.
-  constructor; [| by assert (Z.of_nat multiplier ^ 3 >= 1) by lia].
+  constructor; [| unfold parity_trace1_first_state; cbn;
+                  unfold ParityComponent_initial_state_prop; lia].
   repeat apply ct_extend; [..| apply ct_empty].
   - by apply parity_valid_transition_1.
   - cbn. split; [| lia]. 
@@ -314,17 +318,17 @@ Proof.
 Qed.
 
 Definition parity_trace2_init : list (transition_item ParityVLSM) :=
-  [ Build_transition_item parity_label (Some (Z.of_nat multiplier)) (Z.of_nat multiplier + 1)
-                                       (Some (Z.of_nat multiplier ^ 2))
-  ; Build_transition_item parity_label (Some (Z.of_nat multiplier)) 1 (Some (Z.of_nat multiplier ^ 2)) ].
+  [ Build_transition_item parity_label (Some multiplier) (multiplier + 1)
+                                       (Some (multiplier ^ 2))
+  ; Build_transition_item parity_label (Some multiplier) 1 (Some (multiplier ^ 2)) ].
 
 Definition parity_trace2_last_item : transition_item ParityVLSM :=
-  Build_transition_item parity_label (Some 1) 0 (Some (Z.of_nat multiplier)).
+  Build_transition_item parity_label (Some 1) 0 (Some multiplier).
 
 Definition parity_trace2 : list (transition_item ParityVLSM) :=
   parity_trace2_init ++ [parity_trace2_last_item].
 
-Definition parity_trace2_init_first_state : ParityState := 2 * Z.of_nat multiplier + 1.
+Definition parity_trace2_init_first_state : ParityState := 2 * multiplier + 1.
 
 Definition parity_trace2_init_last_state : ParityState := 1.
 
@@ -334,33 +338,34 @@ Definition parity_trace2_last_state : ParityState := destination parity_trace2_l
 
 Proposition parity_valid_transition_1' :
   input_valid_transition ParityVLSM parity_label
-   (parity_trace2_init_first_state, Some (Z.of_nat multiplier)) (Z.of_nat multiplier + 1, Some (Z.of_nat multiplier ^ 2)).
+   (parity_trace2_init_first_state, Some multiplier) (multiplier + 1, Some (multiplier ^ 2)).
 Proof.
   repeat split; [| | | lia |].
-  - apply initial_state_is_valid.
-    by assert (2 * Z.of_nat multiplier + 1 >= 1) by lia.
+  - unfold parity_trace2_init_first_state; apply initial_state_is_valid; cbn;
+     unfold ParityComponent_initial_state_prop; lia.
   - by app_valid_tran; apply parity_can_emit_square_mult.
   - by unfold parity_trace2_init_first_state; lia.
-  - by cbn; repeat f_equal; unfold parity_trace2_init_first_state; lia.
+  - by cbn; do 2 f_equal; unfold parity_trace2_init_first_state; lia.
 Qed.
 
 Proposition parity_valid_transition_2' :
   input_valid_transition ParityVLSM parity_label
-  (Z.of_nat multiplier + 1, Some (Z.of_nat multiplier)) (1, Some (Z.of_nat multiplier ^ 2)).
+  (multiplier + 1, Some multiplier) (1, Some (multiplier ^ 2)).
 Proof. 
   repeat split; [| | | lia |].
-  - apply initial_state_is_valid.
-    by assert (Z.of_nat multiplier + 1 >= 1) by lia.
+  - unfold parity_trace2_init_first_state; apply initial_state_is_valid; cbn;
+     unfold ParityComponent_initial_state_prop; lia.
   - by app_valid_tran; apply parity_can_emit_square_mult.
   - by unfold parity_trace2_init_first_state; lia.
-  - by cbn; repeat f_equal; unfold parity_trace2_init_first_state; lia.
+  - by cbn; do 2 f_equal; unfold parity_trace2_init_first_state; lia.
 Qed.
 
 Example parity_valid_trace2_init :
   finite_valid_trace_init_to ParityVLSM
    parity_trace2_init_first_state parity_trace2_init_last_state parity_trace2_init.
 Proof.
-  constructor; [| by assert (2 * Z.of_nat multiplier + 1 >= 1) by lia].
+  constructor; [| unfold parity_trace2_init_first_state; cbn;
+                  unfold ParityComponent_initial_state_prop; lia].
   repeat apply finite_valid_trace_from_to_extend.
   - eapply finite_valid_trace_from_to_empty, input_valid_transition_destination, parity_valid_transition_2'.
   - by apply parity_valid_transition_2'.
@@ -371,7 +376,8 @@ Example parity_valid_trace2_init_alt :
   finite_valid_trace_init_to_alt ParityVLSM
    parity_trace2_init_first_state parity_trace2_init_last_state parity_trace2_init.
 Proof.
-  constructor; [| by assert (2 * Z.of_nat multiplier + 1 >= 1) by lia].
+  constructor; [| unfold parity_trace2_init_first_state; cbn;
+                  unfold ParityComponent_initial_state_prop; lia].
   repeat apply mvt_extend; [..| apply mvt_empty].
   - by apply parity_valid_message_prop_mult.
   - by apply parity_valid_transition_1'.
@@ -415,7 +421,7 @@ Proof.
   - by eapply finite_valid_trace_from_to_last_pstate.
   - by apply any_message_is_valid_in_preloaded.
   - by unfold parity_trace2_init_last_state; lia.
-  - by cbn; repeat f_equal; lia.
+  - by cbn; do 2 f_equal; lia.
 Qed.
 
 (** *** Example of a valid transition
@@ -425,12 +431,13 @@ Qed.
 
 Lemma parity_example_valid_transition :
   input_valid_transition ParityVLSM parity_label
-   ((8, 2), Some 2) ((8, 0), Some 4).
+   (multiplier, Some multiplier) (0, Some (multiplier ^ 2)).
 Proof.
-  apply (finite_valid_trace_from_to_last_transition ParityVLSM
-    parity_trace1_first_state parity_trace1_last_state
-    parity_trace1_init parity_trace1 parity_trace1_last_item); [| done].
-  by apply parity_valid_trace1.
+  repeat split; [| | lia.. |].
+  - unfold parity_trace2_init_first_state; apply initial_state_is_valid; cbn;
+     unfold ParityComponent_initial_state_prop; lia.
+  - by apply parity_valid_message_prop_mult.
+  - by cbn; do 2 f_equal; lia.
 Qed.
 
 (** *** Example of a constrained transition
@@ -440,7 +447,7 @@ Qed.
 
 Example parity_example_constrained_transition :
   input_valid_transition (pre_loaded_with_all_messages_vlsm ParityVLSM) parity_label
-   ((5, 1), Some 1) ((5, 0), Some 2).
+   (1, Some 1) (0, Some multiplier).
 Proof.
   apply (finite_valid_trace_from_to_last_transition
     (pre_loaded_with_all_messages_vlsm ParityVLSM)
@@ -463,94 +470,91 @@ Qed.
 
 Lemma parity_constrained_messages_left :
   forall (m : ParityMessage), constrained_message_prop_alt ParityVLSM m ->
-   Z.Even m /\ m > 0.
+   exists (j : Z), m = multiplier * j /\ m > 0.
 Proof.
-  intros m ([s []] & [] & s' & (_ & _ & []) & Ht).
+  intros m Hm.
+  destruct Hm as ([s []] & [] & s' & (_ & _ & []) & Ht).
   inversion Ht; subst.
-  by split; [eexists | lia].
+  by exists p; split; lia.
 Qed.
 
 Lemma parity_constrained_messages_right :
-  forall (m : ParityMessage), Z.Even m -> m > 0 ->
+  forall (m : ParityMessage), (exists (j : Z), m = multiplier * j) -> m > 0 ->
    constrained_message_prop_alt ParityVLSM m.
 Proof.
-  intros m [n ->] Hmgt0.
-  pose (s := (n, n)).
-  exists (s, Some n), parity_label, (n, 0).
-  repeat split.
-  - by apply initial_state_is_valid; constructor; cbn; lia.
+  intros m (j & Hj) Hmgt0.
+  unfold constrained_message_prop_alt, can_emit.
+  exists (j, Some j), parity_label, 0.
+  repeat split; [| | by lia.. | by cbn; do 2 f_equal; lia].
+  - apply input_valid_transition_destination with (l := parity_label) (s := j + 1)
+      (om := Some 1) (om' := Some multiplier).
+    repeat split; [| | lia.. |].
+    + unfold parity_trace2_init_first_state; apply initial_state_is_valid; cbn;
+        unfold ParityComponent_initial_state_prop; lia.
+    + by apply any_message_is_valid_in_preloaded.
+    + cbn; do 2 f_equal; lia.
   - by apply any_message_is_valid_in_preloaded.
-  - by cbn.
-  - by lia.
-  - by cbn; do 2 f_equal; lia.
 Qed.
 
 Lemma parity_constrained_messages :
-  forall (m : ParityMessage),
-   constrained_message_prop_alt ParityVLSM m <-> (Z.Even m /\ m > 0).
+  forall (m : ParityMessage), constrained_message_prop_alt ParityVLSM m <->
+    (exists (j : Z), m = multiplier * j /\ m > 0).
 Proof.
   split.
-  - by apply parity_constrained_messages_left.
-  - by intros [? ?]; apply parity_constrained_messages_right.
+  - apply parity_constrained_messages_left.
+  - by intros [? [? ?]]; apply parity_constrained_messages_right; [exists x |].
 Qed.
 
 (** *** Constrained states property *)
 
 Lemma parity_constrained_states_right :
  forall (st : ParityState),
-  constrained_state_prop_alt ParityVLSM st ->
-   st.1 >= st.2 /\ st.2 >= 0.
+  constrained_state_prop_alt ParityVLSM st -> st >= 0.
 Proof.
   induction 1 using valid_state_prop_ind.
-  - by destruct Hs; lia.
+  - by cbn in Hs; unfold ParityComponent_initial_state_prop in Hs; lia.
   - destruct l, om, Ht as [(Hs & _ & []) Ht].
     by inversion Ht; subst; cbn in *; lia.
 Qed.
 
 Lemma parity_constrained_states_left :
-  forall (st : ParityState), st.1 >= st.2 -> st.2 >= 0 ->
+  forall (st : ParityState), st >= 0 ->
     constrained_state_prop_alt ParityVLSM st.
 Proof.
-  intros st Hn Hi.
-  (* make two cases *)
-  destruct (decide (st.1 = st.2)).
-  - by apply initial_state_is_valid; split; lia.
-  - pose (s := (st.1, st.1)).
-    apply input_valid_transition_destination with (l := parity_label) (s := s)
-      (om := Some (st.1 - st.2)) (om' := Some (2 * (st.1 - st.2))).
-    repeat split.
-    + by apply initial_state_is_valid; constructor; cbn; lia.
-    + by apply any_message_is_valid_in_preloaded.
-    + by unfold s; cbn; lia.
-    + by lia.
-    + by destruct st; cbn; do 2 f_equal; lia.
+  intros st Hst.
+  unfold constrained_state_prop_alt.
+  apply input_valid_transition_destination with (l := parity_label) (s := st + 1)
+    (om := Some 1) (om' := Some multiplier).
+  repeat split; [| | lia.. | cbn; do 2 f_equal; lia].
+  - by apply initial_state_is_valid; cbn; unfold ParityComponent_initial_state_prop; lia.
+  - by apply any_message_is_valid_in_preloaded.
 Qed.
 
 Lemma parity_constrained_states :
   forall (st : ParityState),
-    constrained_state_prop_alt ParityVLSM st <-> (st.1 >= st.2 /\ st.2 >= 0).
+    constrained_state_prop_alt ParityVLSM st <-> (st >= 0).
 Proof.
   split.
   - by apply parity_constrained_states_right.
-  - by intros [? ?]; apply parity_constrained_states_left.
+  - by apply parity_constrained_states_left.
 Qed.
 
 (** *** Powers of 2 greater or equal than 2 are valid messages *)
 
-Lemma parity_valid_messages_powers_of_2_right :
+Lemma parity_valid_messages_powers_of_mult_right :
   forall (m : option ParityMessage),
     option_valid_message_prop ParityVLSM m -> m <> None ->
-      exists p : Z, p >= 1 /\ m = Some (2 ^ p).
+      exists p : Z, p >= 1 /\ m = Some (multiplier ^ p).
 Proof.
   intros m [s Hvsm] Hmnn.
   induction Hvsm using valid_state_message_prop_ind.
   - unfold option_initial_message_prop, from_option in Hom.
     destruct om; [| done].
     unfold initial_message_prop in Hom; cbn in Hom.
-    by exists 1; subst.
+    by exists 1; subst; split; [lia | f_equal; lia].
   - destruct om, IHHvsm2; inversion Ht; cycle 1; [| done ..].
-    inversion H as [Hxgt1 Hs2x].
-    apply Some_inj in Hs2x; subst.
+    inversion H as [Hxgt1 Hsmx].
+    apply Some_inj in Hsmx; subst.
     exists (x + 1).
     rewrite <- Z.pow_succ_r; [f_equal |].
     destruct Hv.
@@ -558,9 +562,9 @@ Proof.
     + by lia.
 Qed.
 
-Lemma parity_valid_messages_powers_of_2_left :
+Lemma parity_valid_messages_powers_of_mult_left :
   forall (p : Z),
-    p >= 1 -> option_valid_message_prop ParityVLSM (Some (2 ^ p)).
+    p >= 1 -> option_valid_message_prop ParityVLSM (Some (multiplier ^ p)).
 Proof.
   intros p Hp.
   assert (0 <= p - 1) by lia.
@@ -569,81 +573,26 @@ Proof.
   clear p Hp Heqx.
   revert x H.
   apply natlike_ind.
-  - by apply initial_message_is_valid.
+  - apply initial_message_is_valid; cbn; unfold ParityComponent_initial_state_prop; lia.
   - intros x Hxgt0 Hindh.
-    pose (msgin := 2 ^ (x + 1)).
-    pose (x' := (msgin, msgin)).
+    pose (msgin := multiplier ^ (x + 1)).
     apply emitted_messages_are_valid.
-    exists (x', Some (2 ^ (x + 1))), parity_label, (x'.1, msgin - msgin); subst x' msgin; cbn.
-    repeat split; [| by apply Hindh | by cbn | by lia |].
-    + by apply initial_state_is_valid; constructor; cbn; lia.
-    + by unfold transition; cbn; rewrite <- Z.pow_succ_r, Z.add_succ_l; [| lia].
+    exists (msgin, Some (multiplier ^ (x + 1))), parity_label, 0. subst msgin; cbn.
+    repeat split.
+    + by apply initial_state_is_valid; cbn; unfold ParityComponent_initial_state_prop; lia.
+    + by apply Hindh.
+    + by lia.
+    + by lia.
+    + cbn; rewrite <- Z.pow_succ_r, Z.add_succ_l; [do 2 f_equal; lia | lia].
 Qed.
 
-Lemma parity_valid_messages_powers_of_2 : forall (om : option ParityMessage),
+Lemma parity_valid_messages_powers_of_mult : forall (om : option ParityMessage),
   om <> None -> ((option_valid_message_prop ParityVLSM om) <->
-    (exists p : Z, p >= 1 /\ om = Some (2 ^ p))).
+    (exists p : Z, p >= 1 /\ om = Some (multiplier ^ p))).
 Proof.
   split.
-  - by intros; apply parity_valid_messages_powers_of_2_right.
-  - by intros (p & Hpgt0 & [= ->]); apply parity_valid_messages_powers_of_2_left.
-Qed.
-
-(** *** Valid states hold non-negative integers of the same parity *)
-
-Lemma parity_valid_states_right :
-  forall (s : ParityState),
-    valid_state_prop ParityVLSM s -> (Z.Even s.2 <-> Z.Even s.1) /\ s.1 >= s.2 /\ s.2 >= 0.
-Proof.
-  induction 1 using valid_state_prop_ind.
-  - destruct Hs as [Hs <-].
-    split; [done | ].
-    by split; lia.
-  - destruct om, l, Ht as [(Hs & Hm & Hv) Ht]; [| done].
-    inversion Ht.
-    destruct Hv as [Hv1 Hv2], IHvalid_state_prop as (Heven & Hgt1 & Hgt2); cbn.
-    apply parity_valid_messages_powers_of_2_right in Hm as [p' (Hpgt0 & [= ->])]; [| auto] .
-    split_and!; [| by lia ..].
-    transitivity (Z.Even s.2); [| done].
-    split.
-    + apply Zeven_sub_preserve_parity.
-      destruct p'; [lia | | lia].
-      exists (2 ^ (Z.pos p - 1)); rewrite <- Z.pow_succ_r; [| lia].
-      by f_equal; lia.
-    + intro Heis.
-      apply Zeven_sub_preserve_parity with (n := s.2); [done |].
-      exists (- 2 ^ (p' - 1)).
-      by rewrite Z.mul_opp_r, <- Z.pow_succ_r, Z.sub_1_r, Z.succ_pred; lia.
-Qed.
-
-Lemma parity_valid_states_left (s : ParityState) :
-  (Z.Even s.2 <-> Z.Even s.1) -> s.1 >= s.2 -> s.2 >= 0 ->
-    valid_state_prop ParityVLSM s.
-Proof.
-  intros Hsameparity Hgt1 Hgt2.
-  apply Zeven_equiv_minus in Hsameparity as [d Hd].
-  assert (d >= 0) by lia.
-  revert s Hgt2 Hgt1 Hd.
-  eapply Zlt_0_ind with (P := fun d => forall s : ParityState, s.2 >= 0 ->
-    s.1 >= s.2 -> s.1 - s.2 = 2 * d -> valid_state_prop ParityVLSM s); [| by lia].
-  intros x Hind _ s Higt0 Hngti Hevendiff.
-  destruct x; [.. | by lia].
-  - by apply initial_state_is_valid; constructor; lia.
-  - apply input_valid_transition_destination
-      with (l := parity_label) (s := (s.1, s.2 + 2)) (om := Some 2) (om' := Some 4).
-    repeat split; cbn; [| | by lia | by lia |].
-    + by eapply Hind with (y := Z.pos p - 1); cbn; lia.
-    + by apply initial_message_is_valid.
-    + by destruct s; cbn; do 2 f_equal; by lia.
-Qed.
-
-Theorem parity_valid_states_same_parity :
-  forall (s : ParityState),
-  valid_state_prop ParityVLSM s <-> ((Z.Even s.2 <-> Z.Even s.1) /\ s.1 >= s.2 /\ s.2 >= 0).
-Proof.
-  split.
-  - by apply parity_valid_states_right.
-  - by intros []; apply parity_valid_states_left; [done | lia ..].
+  - by intros; apply parity_valid_messages_powers_of_mult_right.
+  - by intros (p & Hpgt0 & [= ->]); apply parity_valid_messages_powers_of_mult_left.
 Qed.
 
 End sec_parity_vlsm.
